Accurate.v
@@ -4,3 +4,7 @@ Require Export System.
 Inductive Accurate {msys: MetaSystem} (sys: System msys) : Prop :=
   satisfiesAccuracyRequirement:
     (exists accurate: System msys -> Prop, accurate sys) -> Accurate sys.
+
+Inductive Adaptable {msys: MetaSystem} (sys: System msys) : Prop :=
+  satisfiesAdaptabilityRequirement:
+    (exists adaptable: System msys -> Prop, adaptable sys) -> Adaptable sys.
